LSPLogAnalyzer/Utils.lean
@@ -1,10 +1,12 @@
 import Lean
 import LSPLogAnalyzer.Definitions
 
+open Lean
 open Lean.Json
 open Lean.FromJson
 open Lean.JsonRpc
 open Lean.Lsp
+open Lean.Elab
 
 namespace LSPLogAnalyzer
 
@@ -15,16 +17,22 @@ def fileStream (filename : System.FilePath) : IO Stream := do
 def parseLogLine (line : String) : Except String LogEntry := do
   Lean.fromJson? (← parse line)
 
+def prepareBaseEnv (fname : String) (modName : Lean.Name) : IO Lean.Environment := do
+  let .some env ← runFrontend "" {} fname modName
+    | throw $ IO.userError "unable to create base Environment"
+  return env
+
 def ensureFile (uri : String) : TrackerM FileState := do
   let st ← get
   match st.files.get? uri with
   | some fs => return fs
   | none =>
-    let fs : FileState := {}
+    let baseEnv ← prepareBaseEnv uri `DummyModule
+    let fs : FileState := { baseEnv }
     set { st with files := st.files.insert uri fs }
     return fs
 
-def messageSummary : Message → String
+def messageSummary : JsonRpc.Message → String
   | .request id method@"$/lean/rpc/call" (some params) =>
       let rpcmethod := params.toJson.getObjValAs? String "method" |>.toOption
       s!"request {id} - {method} {rpcmethod.getD "unknown method"}"
@@ -52,28 +60,26 @@ def modifyFileState (uri : Uri) (fs : FileState) : TrackerM Unit := do
 def locatePos (defs : Array Definition) (pos : Lean.Lsp.Position)
     (lo : Nat := 0) (hi : Nat := defs.size) : Option (Nat × Definition) :=
   if hi ≤ lo then none
-  else
+  else do
     let m := (lo + hi) / 2
-    defs[m]? >>= fun d =>
-      if pos ∈ d.range then
-        (m, d)
-      else if pos < d.range.start then
-        locatePos defs pos lo m
-      else
-        locatePos defs pos (m+1) hi
+    let dv ← defs[m]?
+    let r ← dv.range?
+    if      pos ∈ r       then (m, dv)
+    else if pos < r.start then locatePos defs pos lo m
+    else                       locatePos defs pos (m+1) hi
   termination_by hi - lo
 
-def relativePos (origin pos : Position) : Position :=
-  if origin.line == pos.line then
-    ⟨0, pos.character - origin.character⟩
-  else
+def relativePos (origin pos : Lsp.Position) : Lsp.Position :=
+  -- if origin.line == pos.line then
+  --   ⟨0, pos.character - origin.character⟩
+  -- else
     ⟨pos.line - origin.line, pos.character⟩
 
 def relativeRange (enclosing inner : Range) : Range :=
   ⟨relativePos enclosing.start inner.start, relativePos enclosing.start inner.end⟩
 
-def updateDefDiag (defn : Definition) (diag : Diagnostic) : Definition :=
-  let diag := { diag with range := relativeRange defn.range diag.range }
-  { defn with diags := defn.diags.push diag }
+-- def updateDefDiag (defn : Definition) (diag : Diagnostic) : Definition :=
+--   let diag := { diag with range := relativeRange defn.range diag.range }
+--   { defn with diags := defn.diags.push diag }
 
 end LSPLogAnalyzer
