LSPLogAnalyzer/Basic.lean
@@ -23,52 +23,106 @@ def onDidOpen (time : ZonedDateTime) (notif : Notification Lean.Json) : TrackerM
   let .ok (params : LeanDidOpenTextDocumentParams) := fromJson? notif.param
     | onError s!"Unable to parse didOpen parameters {notif.param}"
   let doc := params.textDocument
-  let env ← prepareBaseEnv doc.uri `DummyModule
   let fs ← ensureFile doc.uri
-  let deflikes ← runCollectDefLikes env doc.uri doc.text
-  let fs := { fs with
-    snapshots := fs.snapshots.push ⟨time, doc, #[], #[], deflikes⟩
-    changes := #[] }
+  let defArray ← runCollectDefLikes fs.baseEnv doc
+  let defMap := .ofList <| defArray.toList.map fun d => (d.name.toString, #[d])
+  let snapshots := fs.snapshots.push ⟨time, doc, #[], #[]⟩
+  let fs := { fs with snapshots, defMap, defArray, changes := #[] }
   modifyFileState doc.uri fs
 
 def onDidChange (time : ZonedDateTime) (notif : Notification Lean.Json) : TrackerM Unit := do
   let .ok (params : DidChangeTextDocumentParams) := fromJson? notif.param
-    | onError "Unable to parse didChange parameters {entry.param}"
+    | onError s!"Unable to parse textDocument/didChange parameters {notif.param}"
   let doc := params.textDocument
   let changes := params.contentChanges
   let fs ← ensureFile doc.uri
-  let .some v := doc.version? | onError s!"Missing version in didChange event on line {← getLine}"
+  let .some v := doc.version?
+    | onError s!"Missing version in didChange event on line {← getLine}"
   let fs := { fs with changes := fs.changes.push ⟨time, v, changes⟩}
   modifyFileState doc.uri fs
 
-def updateSnapshot (s : Snapshot) (changes : Array ChangeEvent): Snapshot :=
-  match changes.back? with
-  | none => s
-  | some { time := t, version := v, .. } =>
-    let changes := changes.flatMap (·.changes)
-    let newText := Lean.Server.foldDocumentChanges changes s.doc.text.toFileMap
-    let newdoc := { s.doc with
-      text := newText.source  -- avoid converting back and forth?
-      version := v }
-    {s with doc := newdoc, time := t, goals := #[] }
+def maybeUpdateDefs
+    (defMap : Std.HashMap String (Array Definition))
+    (defArray : Array Definition)
+    : Std.HashMap String (Array Definition) :=
+  defArray.foldl go defMap
+  where
+    go defMap newDef :=
+      defMap.alter newDef.name.toString fun defs? =>
+        match defs? >>= Array.back? with
+        | none => some #[newDef]
+        | some oldDef =>
+            -- TODO : fixme, never pushes anything
+            if newDef.localDiags.all fun d => oldDef.localDiags.any fun d' => d == d' then
+              defs?
+            else
+              let newStx := newDef.defview?.map (·.ref)
+              let oldStx := oldDef.defview?.map (·.ref)
+              if newStx == oldStx then
+                defs? >>= (·.pop.push newDef)
+              else
+                defs? >>= (Array.push · newDef)
 
-def updateDiagnostics (uri : Uri) (fs : FileState) (diags : Array Diagnostic) : TrackerM Unit := do
-  let .some s := fs.snapshots.back? | onError s!"No existing snapshot for {uri} in updateDiagnostics"
-  if s.diags == diags then return
-  let snapshots := match fs.changes with
-  | #[] =>
-    let s := { s with diags := diags }
-    fs.snapshots.pop.push s
-  | changes =>
-    let s := { updateSnapshot s changes with diags := diags }
-    fs.snapshots.push s
-  modifyFileState uri { fs with snapshots := snapshots, changes := #[] }
+def recordLocalDiags
+    (defs : Array Definition)
+    (diags : Array Diagnostic)
+    : (Array Definition × Array Diagnostic) :=
+  diags.foldl go (defs, #[])
+  where
+    go acc diag :=
+      let (res, remainingDiags) := acc
+      let tmp : Option (Nat × LocalDiagnostic) := do
+        let (i, defn) ← locatePos defs diag.range.start
+        let dr ← defn.range?
+        let localRange := relativeRange dr diag.range
+        let localDiag := { diag, localRange }
+        return (i, localDiag)
+      match tmp with
+      | none => (res, remainingDiags.push diag)
+      | some (i, ld) => (res.modify i fun d =>
+        { d with localDiags := d.localDiags.push ld }, remainingDiags)
+
+def normalizeText (text : String) : String :=
+  let lines := text.splitOn "\n"
+    |>.map String.trimRight
+    |>.filter (not ·.isEmpty)
+  "\n".intercalate lines
+
+def updateDiagnostics (uri : Uri) (diags : Array Diagnostic) : TrackerM Unit := do
+  let fs ← ensureFile uri
+  let .some s := fs.snapshots.back?
+    | onError s!"No existing snapshot for {uri} in updateDiagnostics"
+  -- if s.diags == diags then return
+  let (doc, defArray, time, docHasChanged?) ← match fs.changes.back? with
+  | none => pure (s.doc, fs.defArray, s.time, false)
+  | some { time, version, .. } =>
+    let changes := fs.changes.flatMap (·.changes)
+    let newText := Lean.Server.foldDocumentChanges changes s.doc.text.toFileMap
+    if normalizeText newText.source == normalizeText s.doc.text then
+      pure (s.doc, fs.defArray, s.time, false)
+    else
+      -- TODO : avoid converting back and forth?
+      let newdoc := { s.doc with version, text := newText.source }
+      let defArray ← runCollectDefLikes fs.baseEnv newdoc
+      pure (newdoc, defArray, time, true)
+  let (defArray, globalDiags) := recordLocalDiags defArray diags
+  let s := {s with doc := doc, time, globalDiags }
+  let fs := if docHasChanged? then
+    { fs with
+      snapshots := fs.snapshots.push s
+      defArray
+      defMap := maybeUpdateDefs fs.defMap defArray
+      changes := #[] }
+  else
+    { fs with
+      snapshots := fs.snapshots.pop.push s
+      defMap := maybeUpdateDefs fs.defMap defArray }
+  modifyFileState uri fs
 
 def onPublishDiagnostics (notif : Notification Lean.Json) : TrackerM Unit := do
   let .ok (params : PublishDiagnosticsParams) := fromJson? notif.param
     | onError s!"Unable to parse publishDiagnostics parameters {notif.param}"
-  let fs ← ensureFile params.uri
-  updateDiagnostics params.uri fs params.diagnostics
+  updateDiagnostics params.uri params.diagnostics
 
 def onRpcResponse (request : Request Lean.Json) (response : Response Lean.Json) : TrackerM Unit := do
   return
@@ -99,9 +153,10 @@ def processResponse
     (dir : MessageDirection)
     (response : Response Lean.Json) : TrackerM Unit := do
   let ts ← get
-  let .some req := ts.requests.get? response.id | onError s!"Ignored response {response.id} on line {← getLine} (no such pending request)"
+  let .some req := ts.requests.get? response.id
+    | onError s!"Ignored response {response.id} on line {← getLine} (no such pending request)"
   match dir, req.method with
-  | .clientToServer, "$/lean/rpc/call" => onRpcResponse req response
+  -- | .clientToServer, "$/lean/rpc/call" => onRpcResponse req response
   | _, _ => onError s!"Ignored response {response.id} ({req.method}) on line {← getLine}"
   set { ts with requests := ts.requests.erase response.id }
 
